bunch of stuff

theories/equivalence/types.v
@@ -69,6 +69,12 @@ Qed.
 
 (* boring properties about closedness {{{ *)
 
+Lemma subst_through_arrow {τ1 τ2} σ : (TArrow τ1 τ2).[σ] = TArrow τ1.[σ] τ2.[σ].
+Proof. by asimpl. Qed.
+
+Lemma subst_through_rec {τb} σ : (TRec τb).[σ] = TRec τb.[up σ].
+Proof. by asimpl. Qed.
+
 Lemma TArrow_closed1 {τ1 τ2} : TClosed (TArrow τ1 τ2) → TClosed τ1.
 Proof.
   unfold TClosed.
@@ -103,17 +109,6 @@ Proof.
   done.
 Qed.
 
-Lemma TRec_closed_unfold_pre {τ τ'} : TClosed (TRec τ) → TClosed τ' → TClosed (τ.[τ'/]).
-Proof.
-  intros.
-  induction τ.
-  - by asimpl.
-  - asimpl. apply TArrow_closed. apply IHτ1. admit.
-Admitted.
-
-Lemma TRec_closed_unfold {τ} : TClosed (TRec τ) → TClosed (τ.[TRec τ/]).
-Proof. intro; by apply TRec_closed_unfold_pre. Qed.
-
 Lemma no_var_is_closed x : not (TClosed (TVar x)).
 Proof.
   intro H. assert (abs : (TVar x).[ren (+1)] = TVar x); first by apply H.
@@ -125,13 +120,16 @@ Qed.
 
 (* boring properties about substitution {{{ *)
 
+Lemma scomp_comp (σ1 σ2 : var → type) τ : (subst σ1 ∘ subst σ2) τ = subst (σ2 >> σ1) τ.
+Proof. by asimpl. Qed.
+
 Lemma scomp_assoc (σ1 σ2 σ3 : var → type) : (σ1 >> σ2) >> σ3 = σ1 >> (σ2 >> σ3).
 Proof. by asimpl. Qed.
 
-Lemma subst_commut (τ τ' : type) (σ : var → type) : up σ >> scons (τ.[σ]) ids = scons τ ids >> σ.
+Lemma subst_commut (τ : type) (σ : var → type) : up σ >> scons (τ.[σ]) ids = scons τ ids >> σ.
 Proof. by asimpl. Qed.
 
-Lemma subst_fv n m σ : (TVar (n + m)).[upn n σ] = ((TVar m).[σ].[ren (+n)]).
+Lemma subst_fv_upn_yes n m σ : (TVar (n + m)).[upn n σ] = ((TVar m).[σ].[ren (+n)]).
 Proof.
   asimpl.
   induction n.
@@ -139,8 +137,142 @@ Proof.
   - asimpl. rewrite IHn. by asimpl.
 Qed.
 
-Lemma subst_fv_no n m σ : n < m → (TVar n).[upn m σ] = TVar n.
+Lemma subst_fv_upn_no n m σ : n < m → (TVar n).[upn m σ] = TVar n.
 Proof.
-Admitted.
+  generalize dependent n.
+  induction m.
+  - intros. exfalso. lia.
+  - intros. destruct n.
+    + by asimpl.
+    + asimpl. asimpl in IHm. rewrite IHm. by asimpl. lia.
+Qed.
+
+Lemma subst_fv_upn_cases k n σ : ((TVar k).[upn n σ] = TVar k ∧ k < n) +
+                                 { j : nat | k = n + j ∧ (TVar k).[upn n σ] = (TVar j).[σ].[ren (+n)]  }.
+Proof.
+  destruct (decide (k < n)).
+  - apply inl. split. apply subst_fv_upn_no; auto. auto.
+  - apply inr. exists (k - n). split. lia. rewrite -subst_fv_upn_yes.
+    assert (triv : k = n + (k - n)). lia. by rewrite -triv.
+Qed.
+
 
 (* }}} *)
+
+Definition TnClosed : nat → type → Prop := fun n τ => forall σ, τ.[upn n σ] = τ.
+
+Lemma TArrow_nclosed1 {τ1 τ2} {n} : TnClosed n (TArrow τ1 τ2) → TnClosed n τ1.
+Proof.
+  unfold TnClosed.
+  intros H σ.
+  assert (H' : TArrow τ1.[upn n σ] τ2.[upn n σ] = TArrow τ1 τ2). asimpl in H. by rewrite H.
+  inversion H'.
+  by do 2 rewrite H1.
+Qed.
+
+Lemma TArrow_nclosed2 {τ1 τ2} {n} : TnClosed n (TArrow τ1 τ2) → TnClosed n τ2.
+Proof.
+  unfold TnClosed.
+  intros H σ.
+  assert (H' : TArrow τ1.[upn n σ] τ2.[upn n σ] = TArrow τ1 τ2). asimpl in H; by rewrite H.
+  inversion H'.
+  by do 2 rewrite H2.
+Qed.
+
+Lemma TArrow_nclosed {τ1 τ2} {n} : (TnClosed n τ1 ∧ TnClosed n τ2) ↔ TnClosed n (TArrow τ1 τ2).
+Proof.
+  split. intros (H1, H2). intro σ. asimpl. by rewrite H1 H2.
+  intros. split. by eapply TArrow_nclosed1. by eapply TArrow_nclosed2.
+Qed.
+
+Lemma TRec_nclosed1 {τ} {n} : TnClosed n (TRec τ) → TnClosed (S n) τ.
+Proof.
+  intros H σ.
+  assert (H' : TRec τ.[upn (S n) σ] = TRec τ). specialize (H σ). by asimpl in H.
+  inversion H'.
+  by do 2 rewrite H1.
+Qed.
+
+Lemma TRec_nclosed {τ} {n} : TnClosed n (TRec τ) ↔ TnClosed (S n) τ.
+Proof.
+  split. apply TRec_nclosed1.
+  intros H σ.
+  asimpl. apply f_equal. apply H.
+Qed.
+
+Lemma TnClosed_var (x n : nat) : TnClosed n (TVar x) ↔ x < n.
+Proof.
+  split.
+  - intros.
+    destruct (subst_fv_upn_cases x n (ren (+1))) as [[_ eq] | [j [-> _]]].
+    + auto.
+    + exfalso. unfold TnClosed in H.
+      specialize (H (ren (+1))).
+      rewrite subst_fv_upn_yes in H.
+      asimpl in H. inversion H. lia.
+  - intros. intro σ. by apply subst_fv_upn_no.
+Qed.
+
+Lemma le_exists_add x y : x ≤ y → exists z, x + z = y.
+Proof. intros. exists (y - x). lia. Qed.
+
+Lemma TnClosed_mon τ (n m : nat) : n ≤ m → TnClosed n τ → TnClosed m τ.
+Proof.
+  intros ple pnτ. intro σ. destruct (le_exists_add n m ple) as [z <-]. generalize σ. clear σ.
+  simpl. induction z. asimpl. intro σ. by rewrite pnτ. intro σ. cut (τ.[upn (n + S z) σ] = τ.[upn (n + z) (up σ)]).
+  intro. rewrite H. apply IHz. lia. by asimpl.
+Qed.
+
+Lemma TnClosed_ren_gen (τ : type) :
+  forall (n m : nat) (pτ : TnClosed n τ) (l : nat), TnClosed (m + n) τ.[upn l (ren (+m))].
+Proof.
+  induction τ; intros.
+  - by asimpl.
+  - specialize (IHτ1 n m ltac:(by eapply TArrow_nclosed1) l).
+    specialize (IHτ2 n m ltac:(by eapply TArrow_nclosed2) l).
+    simpl. intro σ. simpl. by rewrite IHτ1 IHτ2.
+  - rewrite subst_through_rec.
+    apply TRec_nclosed.
+    specialize (IHτ (S n) m ltac:(by apply TRec_nclosed) (S l)).
+    by asimpl in *.
+  - destruct (subst_fv_upn_cases x l (ren (+m))) as [[-> p] | [j [eq ->]]].
+    + eapply (TnClosed_mon _ n). lia. apply pτ.
+    + asimpl. apply TnClosed_var.
+      assert (H : x < n). by apply TnClosed_var. lia.
+  - by asimpl.
+Qed.
+
+Lemma TnClosed_ren (τ : type) :
+  forall (n m : nat) (pτ : TnClosed n τ), TnClosed (m + n) τ.[ren (+m)].
+Proof. intros. cut (TnClosed (m + n) τ.[upn 0 (ren (+m))]). by asimpl. by apply TnClosed_ren_gen. Qed.
+
+Lemma TnClosed_subst_gen n τ τ' : forall m, TnClosed (S (m + n)) τ' → TnClosed n τ → TnClosed ((m + n)) τ'.[upn m (τ .: ids)].
+Proof.
+  generalize dependent n.
+  induction τ'; intros.
+  - asimpl. intro σ; by asimpl.
+  - asimpl.
+    specialize (IHτ'1 n m ltac:(by eapply TArrow_nclosed1) H0).
+    specialize (IHτ'2 n m ltac:(by eapply TArrow_nclosed2) H0).
+    intro σ. simpl. by rewrite IHτ'1 IHτ'2.
+  - simpl.
+    apply TRec_nclosed.
+    apply (IHτ' n (S m)). by apply TRec_nclosed. auto.
+  - destruct (subst_fv_upn_cases x m (τ .: ids)) as [[-> p] | [j [eq ->]]].
+    + apply TnClosed_var. lia.
+    + destruct j.
+      * asimpl. by apply TnClosed_ren.
+      * asimpl. assert (p1 : x < S (m + n)). by apply TnClosed_var.
+        apply TnClosed_var. lia.
+  - by asimpl.
+Qed.
+
+Lemma TnClosed_subst n τ τ' : TnClosed (S n) τ' → TnClosed n τ → TnClosed n τ'.[τ/].
+Proof. intros. rewrite -(upn0 (τ .: ids)). apply (TnClosed_subst_gen n τ τ' 0); auto. Qed.
+
+(* Lemma TRec_closed_unfold_pre {τ τ'} : TClosed (TRec τ) → TClosed τ' → TClosed (τ.[τ'/]). *)
+
+Lemma TRec_closed_unfold {τ} : TClosed (TRec τ) → TClosed (τ.[TRec τ/]).
+Proof. intro. cut (TnClosed 0 τ.[TRec τ/]). by simpl. apply TnClosed_subst.
+       apply TRec_nclosed. by simpl. by simpl.
+Qed.
