theories/equivalence/upper_bound.v
@@ -1,31 +1,48 @@
-From fae_gtlc_mu.equivalence Require Import types closures.
+From fae_gtlc_mu.equivalence Require Import types closed_rec_types listset_ext.
 From stdpp Require Import base listset.
 From iris Require Import base.
 
-Definition combinations (τ τ' : type) : list (type * type) := (* we count more then actually possible but no biggie *)
-  list_prod (closures τ) [TRec TUnknown] ++
-  list_prod [TRec TUnknown] (closures τ) ++
-  list_prod (closures τ') [TRec TUnknown] ++
-  list_prod [TRec TUnknown] (closures τ') ++
-  list_prod (closures τ) (closures τ') ++
-  list_prod (closures τ') (closures τ).
+Definition combinations (τ τ' : type) : listset (type * type) := (* we count more then actually possible but no biggie *)
+  listset_prod (closed_rec_types τ) {[TRec TUnknown]} ∪
+  listset_prod (closed_rec_types τ') {[TRec TUnknown]} ∪
+  listset_prod {[TRec TUnknown]} (closed_rec_types τ) ∪
+  listset_prod {[TRec TUnknown]} (closed_rec_types τ') ∪
+  listset_prod (closed_rec_types τ) (closed_rec_types τ') ∪
+  listset_prod (closed_rec_types τ') (closed_rec_types τ).
 
 Notation "{{ l }}" := (Listset l) (at level 20).
 
 Definition upper_bound (A : list (type * type)) τ τ' : nat :=
-  size ({{combinations τ τ'}} ∖ {{A}}).
+  size (combinations τ τ' ∖ {{A}}).
 
 Notation "#" := upper_bound.
 
-(** if types are structurally smaller, then upper_bound is smaller or equal *)
+Lemma subseteq_comp_normal {X1 X1' X2 X2' X3 X3' X4 X4' X5 X5' X6 X6' : listset (type * type)}
+      (H1 : X1 ⊆ X1') (H2 : X2 ⊆ X2') (H3 : X3 ⊆ X3') (H4 : X4 ⊆ X4') (H5 : X5 ⊆ X5') (H6 : X6 ⊆ X6') :
+  X1 ∪ X2 ∪ X3 ∪ X4 ∪ X5 ∪ X6 ⊆ X1' ∪ X2' ∪ X3' ∪ X4' ∪ X5' ∪ X6'.
+Proof. set_solver. Qed.
 
-Lemma upper_bound_le_arrow_l A τ1 τ2 τ1' τ2' :
-  # A τ1' τ1 ≤ # A (TArrow τ1 τ2) (TArrow τ1' τ2').
+Lemma subseteq_comp_contravariant {X1 X1' X2 X2' X3 X3' X4 X4' X5 X5' X6 X6' : listset (type * type)}
+      (H1 : X1 ⊆ X2') (H2 : X2 ⊆ X1') (H3 : X3 ⊆ X4') (H4 : X4 ⊆ X3') (H5 : X5 ⊆ X6') (H6 : X6 ⊆ X5') :
+  X1 ∪ X2 ∪ X3 ∪ X4 ∪ X5 ∪ X6 ⊆ X1' ∪ X2' ∪ X3' ∪ X4' ∪ X5' ∪ X6'.
+Proof. set_solver. Qed.
+
+Lemma size_elem_difference_suc {A : Type} {_ : EqDecision A} (l : listset A) (k : list A) (a : A) : a ∈ l → a ∉ k →
+  size (l ∖ {{k}}) = S (size (l ∖ {{a :: k}})).
 Proof.
-  rewrite /upper_bound.
-  apply subseteq_size.
-  apply difference_mono_r.
-Admitted.
+  intros.
+  assert (triv : l ≡ l ∖ {[a]} ∪ {[a]}).
+  { apply set_subseteq_antisymm; try set_solver.
+    intros τ pin; destruct (decide (τ = a)); set_solver. } rewrite{1} triv. clear triv.
+  rewrite difference_union_distr_l.
+  rewrite size_union_alt.
+  assert (triv : {[a]} ≡ {[a]} ∖ {{k}} ∖ (l ∖ {[a]} ∖ {{k}})). set_solver. rewrite -triv. clear triv.
+  assert (triv : l ∖ {[a]} ∖ {{k}} ≡ l ∖ {{a :: k}}).
+  { assert (triv : {{a :: k}} = {[a]} ∪ {{k}}). set_solver. rewrite triv. clear triv. set_solver. } rewrite triv. clear triv.
+  rewrite size_singleton. lia.
+Qed.
+
+(** if types are structurally smaller, then upper_bound is smaller or equal *)
 
 Lemma upper_bound_le_arrow_r A τ1 τ2 τ1' τ2' :
   # A τ2 τ2' ≤ # A (TArrow τ1 τ2) (TArrow τ1' τ2').
@@ -33,22 +50,55 @@ Proof.
   rewrite /upper_bound.
   apply subseteq_size.
   apply difference_mono_r.
-Admitted.
+  apply subseteq_comp_normal; apply listset_prod_subseteq; set_solver.
+Qed.
+
+Lemma upper_bound_le_arrow_l A τ1 τ2 τ1' τ2' :
+  # A τ1' τ1 ≤ # A (TArrow τ1 τ2) (TArrow τ1' τ2').
+Proof.
+  rewrite /upper_bound.
+  apply subseteq_size.
+  apply difference_mono_r.
+  rewrite /combinations.
+  apply subseteq_comp_contravariant; apply listset_prod_subseteq; set_solver.
+Qed.
 
 (** if types is structurally larger, i.e. from i.e. τb.[μ.τb/] > μ.τ,
     then upper_bound is smaller *)
 
-Lemma upper_bound_lt_rec_star A τb (pn : (TRec τb, TRec TUnknown) ∉ A) :
+Lemma upper_bound_lt_rec_star A τb (pμτb : TClosed (TRec τb)) (pn : (TRec τb, TRec TUnknown) ∉ A) :
   # ((TRec τb, TRec TUnknown) :: A) τb.[TRec τb/] TUnknown < # A (TRec τb) TUnknown.
 Proof.
-Admitted.
+  rewrite /upper_bound.
+  rewrite (size_elem_difference_suc _ A (TRec τb, TRec TUnknown)); try auto.
+  + apply le_lt_n_Sm. apply subseteq_size. apply difference_mono_r.
+    apply subseteq_comp_normal; apply listset_prod_subseteq; (apply (closed_rec_types_unfold_subset τb pμτb) || set_solver).
+  + rewrite /combinations.
+    cut ((TRec τb, TRec TUnknown) ∈ listset_prod (closed_rec_types (TRec τb)) {[TRec TUnknown]}). set_solver.
+    apply in_listset_prod_iff; set_solver.
+Qed.
 
-Lemma upper_bound_lt_star_rec A τb (pn : (TRec TUnknown, TRec τb) ∉ A) :
+Lemma upper_bound_lt_star_rec A τb (pμτb : TClosed (TRec τb)) (pn : (TRec TUnknown, TRec τb) ∉ A) :
   # ((TRec TUnknown, TRec τb) :: A) TUnknown τb.[TRec τb/] < # A TUnknown (TRec τb).
 Proof.
-Admitted.
+  rewrite /upper_bound.
+  rewrite (size_elem_difference_suc _ A (TRec TUnknown, TRec τb)); try auto.
+  + apply le_lt_n_Sm. apply subseteq_size. apply difference_mono_r.
+    (* apply closed_rec_types_unfold_subset. *)
+    apply subseteq_comp_normal; apply listset_prod_subseteq; (apply (closed_rec_types_unfold_subset τb pμτb) || set_solver).
+  + rewrite /combinations.
+    cut ((TRec TUnknown, TRec τb) ∈ listset_prod {[TRec TUnknown]} (closed_rec_types (TRec τb))). set_solver.
+    apply in_listset_prod_iff; set_solver.
+Qed.
 
-Lemma upper_bound_lt_rec_rec A τb τb' (pn : (TRec τb, TRec τb') ∉ A) :
+Lemma upper_bound_lt_rec_rec A τb (pμτb : TClosed (TRec τb)) τb' (pμτb' : TClosed (TRec τb')) (pn : (TRec τb, TRec τb') ∉ A) :
   # ((TRec τb, TRec τb') :: A) τb.[TRec τb/] τb'.[TRec τb'/] < # A (TRec τb) (TRec τb').
 Proof.
-Admitted.
+  rewrite /upper_bound.
+  rewrite (size_elem_difference_suc _ A (TRec τb, TRec τb')); try auto.
+  + apply le_lt_n_Sm. apply subseteq_size. apply difference_mono_r.
+    apply subseteq_comp_normal; apply listset_prod_subseteq; (by eapply (closed_rec_types_unfold_subset) || set_solver).
+  + rewrite /combinations.
+    cut ((TRec τb, TRec τb') ∈ listset_prod (closed_rec_types (TRec τb)) (closed_rec_types (TRec τb'))). set_solver.
+    apply in_listset_prod_iff; set_solver.
+Qed.
