theories/backtranslation/well_typedness.v
@@ -1,0 +1,70 @@
+From fae_gtlc_mu.cast_calculus Require Export typing contexts.
+From fae_gtlc_mu.stlc_mu Require Export typing contexts.
+
+From fae_gtlc_mu.backtranslation Require Import types expressions cast_help.general contexts.
+
+Lemma well_typedness_expr Γ e τ :
+  Γ ⊢ₜ e : τ →
+    map backtranslate_type Γ ⊢ₛ backtranslate_expr e : backtranslate_type τ.
+Proof.
+  induction 1; simpl; try by constructor.
+  - constructor. by rewrite list_lookup_fmap H.
+  - eapply Fst_typed. apply IHtyped.
+  - eapply Snd_typed. apply IHtyped.
+  - eapply Case_typed. apply IHtyped1. apply IHtyped2. apply IHtyped3.
+  - eapply App_typed. apply IHtyped1. apply IHtyped2.
+  - apply Fold_typed.
+    rewrite unfolding_backtranslation_commutes in IHtyped.
+    apply IHtyped.
+  - rewrite unfolding_backtranslation_commutes.
+    apply Unfold_typed. apply IHtyped.
+  - destruct (cons_stand_dec τi τf); destruct (decide (TClosed τi)); destruct (decide (TClosed τf)); try by contradiction.
+    eapply App_typed.
+    rewrite /𝓕c /env_subst. admit.
+    apply IHtyped.
+  - apply Ω_typed. admit.
+Admitted.
+
+From fae_gtlc_mu.embedding Require Export types.
+
+Lemma well_typedness_ctx_item Γ τ Γ' τ' C :
+  cast_calculus.contexts.typed_ctx_item C Γ τ Γ' τ' →
+  typed_ctx_item (backtranslate_ctx_item C) (map backtranslate_type Γ) (backtranslate_type τ) (map backtranslate_type Γ') (backtranslate_type τ').
+Proof.
+  induction 1; try (by constructor).
+  - apply TP_CTX_AppL. apply well_typedness_expr; done.
+  - apply TP_CTX_AppR.
+    assert (triv : backtranslate_type (types.TArrow τ τ') = TArrow <<τ>> <<τ'>>). by simpl. rewrite -triv. clear triv.
+    by apply well_typedness_expr.
+  - constructor. by apply well_typedness_expr.
+  - constructor. by apply well_typedness_expr.
+  - constructor.
+    assert (triv : backtranslate_type τ1 :: (map backtranslate_type Γ) = map backtranslate_type (τ1 :: Γ)). by simpl. rewrite triv. clear triv.
+      by apply well_typedness_expr.
+    assert (triv : backtranslate_type τ2 :: (map backtranslate_type Γ) = map backtranslate_type (τ2 :: Γ)). by simpl. rewrite triv. clear triv.
+      by apply well_typedness_expr.
+  - apply TP_CTX_CaseM with (τ2 := <<τ2>>).
+    assert (triv : backtranslate_type (types.TSum τ1 τ2) = TSum <<τ1>> <<τ2>>). by simpl. rewrite -triv. clear triv.
+      by apply well_typedness_expr.
+    assert (triv : backtranslate_type τ2 :: (map backtranslate_type Γ) = map backtranslate_type (τ2 :: Γ)). by simpl. rewrite triv. clear triv.
+      by apply well_typedness_expr.
+  - apply TP_CTX_CaseR with (τ1 := <<τ1>>).
+    assert (triv : backtranslate_type (types.TSum τ1 τ2) = TSum <<τ1>> <<τ2>>). by simpl. rewrite -triv. clear triv.
+      by apply well_typedness_expr.
+    assert (triv : backtranslate_type τ1 :: (map backtranslate_type Γ) = map backtranslate_type (τ1 :: Γ)). by simpl. rewrite triv. clear triv.
+      by apply well_typedness_expr.
+  - rewrite unfolding_backtranslation_commutes. apply TP_CTX_Fold.
+  - rewrite unfolding_backtranslation_commutes. apply TP_CTX_Unfold.
+  - simpl. destruct (cons_stand_dec τi τf); destruct (decide (TClosed τi)); destruct (decide (TClosed τf)); try by contradiction.
+    eapply TP_CTX_AppR. admit.
+Admitted.
+
+Lemma well_typedness_ctx Γ τ Γ' τ' C :
+  cast_calculus.contexts.typed_ctx C Γ τ Γ' τ' →
+  typed_ctx (backtranslate_ctx C) (map backtranslate_type Γ) (backtranslate_type τ) (map backtranslate_type Γ') (backtranslate_type τ').
+Proof.
+  induction 1.
+  - constructor.
+  - econstructor; simpl. by apply well_typedness_ctx_item.
+    auto.
+Qed.
