theories/equivalence/listset_ext.v
@@ -1,0 +1,63 @@
+From iris Require Export base.
+From stdpp Require Export base list sets mapset.
+From stdpp Require Export base.
+(* From stdpp Require Import base binders boolset coGset coPset countable decidable finite fin_map_dom fin_maps fin_sets fin functions gmap gmultiset hashset hlist infinite lexico listset_nodup listset list mapset namespaces nat_cancel natmap nmap numbers option orders pmap pretty proof_irrel propset relations sets sorting streams stringmap strings tactics telescopes vector. *)
+(* fhin_sets fin_maps. *)
+From Autosubst Require Export Autosubst.
+Require Export Utf8_core.
+From fae_gtlc_mu.equivalence Require Import types.
+
+Lemma map_union {A B} (l k : listset A) (f : A → B) : f <$> (l ∪ k) ≡ (f <$> l) ∪ (f <$> k).
+Proof. set_solver. Qed.
+
+Lemma map_singleton {A B} (a : A) (f : A → B) : (f <$> ({[ a ]} : listset A)) ≡ {[ (f a) ]}.
+Proof. set_solver. Qed.
+
+Lemma set_Forall_fmap_ext_1 (f g : type → type) (X : listset type) :
+  set_Forall (λ x : type, f x = g x) X → f <$> X ≡ g <$> X.
+Proof.
+  intro.
+  apply set_subseteq_antisymm.
+  + intros τ Hτ.
+    destruct (elem_of_fmap_1 _ _ _ Hτ) as [τ' [-> pin]].
+    assert (Heq : f τ' = g τ'). apply H. apply  pin. rewrite Heq.
+      by apply elem_of_fmap_2.
+  + intros τ Hτ.
+    destruct (elem_of_fmap_1 _ _ _ Hτ) as [τ' [-> pin]].
+    assert (Heq : f τ' = g τ'). apply H. apply  pin. rewrite -Heq.
+      by apply elem_of_fmap_2.
+Qed.
+
+Lemma set_Forall_subseteq (X Y : listset type) (P : type → Prop) :
+  X ⊆ Y → set_Forall P Y → set_Forall P X.
+Proof. intros. intros τ Hτ. apply H0. set_solver. Qed.
+
+Lemma fmap_listset_id (X : listset type) :
+  id <$> X ≡ X.
+Proof. set_solver. Qed.
+
+Lemma set_Forall_fmap_impl (f : type → type) (X : listset type) (P Q : type → Prop)
+      (Himpl : forall τ : type, P τ → Q (f τ)) (HP : set_Forall P X) : set_Forall Q (f <$> X).
+Proof.
+  intros τ Hτ.
+  destruct (elem_of_fmap_1 _ _ _ Hτ) as [τ' [-> pin]].
+  apply Himpl. by apply HP.
+Qed.
+
+Definition listset_prod {A B : Type} (k : listset A) (l : listset B) : listset (A * B) :=
+  Listset $ list_prod (listset_car k) (listset_car l).
+
+Lemma in_listset_prod_iff {A B : Type} (l : listset A) (l' : listset B) (x : A) (y : B) :
+  (x, y) ∈ (listset_prod l l') ↔ x ∈ l ∧ y ∈ l'.
+Proof.
+  rewrite /elem_of /listset_elem_of. do 3 rewrite elem_of_list_In.
+  simpl. apply in_prod_iff.
+Qed.
+
+Lemma listset_prod_subseteq {A : Type} (k k' l l' : listset A) :
+  k ⊆ k' → l ⊆ l' → listset_prod k l ⊆ listset_prod k' l'.
+Proof.
+  intros. intros (x , y) Hxy. apply in_listset_prod_iff.
+  cut (x ∈ k ∧ y ∈ l). set_solver.
+  by apply in_listset_prod_iff.
+Qed.
